Weidenbach_Book/IsaSAT_Initialisation_LLVM.thy
@@ -616,10 +616,10 @@ sepref_def finalise_init_code'
   apply (rewrite at \<open>(_, \<hole>, _)\<close> al_fold_custom_empty[where 'l=64])
   apply (rewrite at \<open>(_, \<hole>)\<close> al_fold_custom_empty[where 'l=64])
   apply (rewrite in \<open>take _ \<hole>\<close> al_fold_custom_replicate)
-  apply (rewrite at \<open>replicate _ False\<close> annotate_assn[where A=phase_saver_assn])
-  apply (rewrite in \<open>replicate _ False\<close> larray_fold_custom_replicate)
-  apply (rewrite at \<open>replicate _ False\<close> annotate_assn[where A=phase_saver_assn])
-  apply (rewrite in \<open>replicate _ False\<close> larray_fold_custom_replicate)
+  apply (rewrite at \<open>replicate _ False\<close> annotate_assn[where A=phase_saver'_assn])
+  apply (rewrite in \<open>replicate _ False\<close> array_fold_custom_replicate)
+  apply (rewrite at \<open>replicate _ False\<close> annotate_assn[where A=phase_saver'_assn])
+  apply (rewrite in \<open>replicate _ False\<close> array_fold_custom_replicate)
   by sepref
 
 declare finalise_init_code'.refine[sepref_fr_rules]
